% !TeX spellcheck = en_US
\documentclass[week=11]{homework}
\usepackage{scrextend}
\date{\today}


\begin{document}
    \maketitle
    \thispagestyle{empty}
    \newpage
    \begin{questions}
		\let\firstquestion\question
		\renewcommand*{\question}{\vspace{7mm}\firstquestion}
        \firstquestion
		Let $\{b_n \}$ be a sequence of numbers. 
		\begin{inlinetoprove}
			If $\{b_n \}$ converges, then 
			\[
				\limsup b_n = \lim_{n \to \infty} b_n.
			\]
		\end{inlinetoprove}
		\begin{proof}
			First of all, we know that $b_n$ converges. Therefore:
			\[
				\exists_{b^*}: b_n \to b^*
			\]
			Now, because $b_n$ converges, this sequence only has one accumulation point, namely $b^*$. Therefore, the set of all accumulation points of $b_n$, which we call V, only consists of one point: 
			\[
				V = \{b^*\}
			\]
			Now, we can find $\limsup b_n$:
			\[
				\limsup b_n = \sup V = b^*
			\]
			We also know that:
			\[
				\lim_{n \to \infty} b_n = b^*
			\]
			Now, we have proven that:
			\[
				\limsup b_n = \lim_{n \to \infty} b_n
			\]
		\end{proof}
		\question
		Let $\{b_n \}$ and $\{c_n \}$ be a sequences of numbers with $c_n \to 1$. 
		\begin{inlinetoprove}
			\[
				\limsup (c_n b_n) = \limsup b_n, \quad \limsup (b_n^{c_n}) = \limsup b_n
			\]
		\end{inlinetoprove}
		
		\question
		Let R be the radius of convergence for $\sum_{k=0}^{\infty} a_k (x - a)^k$ and suppose that $\lim_{n \to \infty} \left| \frac{a_{n+1}}{a_n} \right| = L$. Then:
		\begin{parts}
			\part if $L$ is a nonzero finite real number, $R = \frac{1}{L}$
			\part if $L=0$, $R = \infty$
			\part if $L = \infty$, $R = 0$. 
		\end{parts}
		
		\question
		Find both the radius and interval of convergence for the given series. Also, determine the values of x for which the series converges absolutely and those for which the series converges conditionally. 
		\begin{parts}
			\part $\sum_{k=1}^{\infty} k(x-2)^k$
			\part $\sum_{k=1}^{\infty} \frac{1}{k} \left( \frac{x}{2} \right)^k$
			\part $\sum_{k=0}^{\infty} k \left( -\frac{1}{3} \right)^k (x-2)^k $
			\part $\sum_{k=1}^{\infty} \frac{2^k k!}{k^k} x^k$
			\part $\sum_{k=0}^{\infty} \frac{k}{3^{2k-1}} (x-1)^{2k}$
		\end{parts}
     \end{questions}
\end{document}