
% !TeX spellcheck = en_US
\documentclass[week=11]{homework}

\date{\today}


\begin{document}
	\maketitle
	\thispagestyle{empty}
	\newpage
	\begin{questions}
		\let\firstquestion\question
		\renewcommand*{\question}{\vspace{7mm}\firstquestion}
		\firstquestion
		Let $D \subset \reals$ unbounded above and let $(f_n)$ be a function sequence on $D$ that converges uniform to a function $f^*$. Assume that 
		\[
			\lim_{x \to \infty} f_n(x) = L_n \quad and \quad \lim_{n \to \infty} L_n = L^* 
		\]
		\begin{toprove}
			$\lim_{x \to \infty} f^*(x) = L^*$
		\end{toprove}
		\begin{proof}
			We know three things:
			\begin{itemize}
				\item $f_n \to f^*$ uniform
				
				\[
					\forall_{\epsilon > 0} \exists_{n_0} \forall_{n \ge n_0} \forall_{x \in D}: |f_x - f^*| < \frac{\epsilon}{3}
				\]
				
				\item  $\lim_{x \to \infty} f_n(x) = L_n$
				
				\[
					\forall_{\epsilon > 0} \exists_{x_0} \forall_{x \in D} : x \ge x_0 \Rightarrow |f_n(x) - L_n| < \frac{\epsilon}{3}
				\]
				\item  $\lim_{n \to \infty} L_n = L^*$
				
				\[
					\forall_{\epsilon > 0} \exists_{n_1} \forall_{n \ge n_1} : |L_n - L^*| < \frac{\epsilon}{3}
				\] 
			\end{itemize}
			
			Let $\epsilon > 0$ be given. Define $n^* = \max\{n_0, n_1\}$. Now let $n \ge n^*$ and $x \ge x_0$. Then:
			\begin{align*}
				|f^*(x) - L^*| &\le |f_n - f^*| + |f_n - L^*|  \\
				&\le |f_n - f^*| + |f_n - f^*| + |L_n - L^*| \\
				&< \frac{\epsilon}{3} + \frac{\epsilon}{3} + \frac{\epsilon}{3} = \epsilon
			\end{align*}
		\end{proof}
		
		\question 
		Use $\frac{1}{1 - x} = 1 + x + x^2 + x^3 + ...$ if $|x| < 1$ to find a series representation for 
		\begin{parts}
			\part \label{5a}$f(x) = \frac{1}{1 - 2x}$			
			\[
				f(x) = \frac{1}{1 - 2x} = \sum (2x)^k
			\]
			
			\part $f(x) = \frac{1}{x}$			
			Take $x = 1-u$. Now:
			\[
				f(x) = \frac{1}{x} = \frac{1}{1-u} = \sum (u)^k = \sum (1-x)^k
			\]
			
			\part $f(x) = \frac{a}{x - b}$ with $a$ and $b$ positive real constants. 			
			\begin{align*}
				f(x) &= \frac{a}{x - b} \\
				&= a \cdot \frac{1}{x - b} \\
				&= \frac{a}{b} \cdot \frac{1}{\frac{x}{b} - 1} \\
				&= -\frac{a}{b} \cdot \frac{1}{1 - \frac{x}{b}} \\
				&= - \frac{a}{b} \cdot \sum \left(\frac{x}{b} \right)^k 
			\end{align*}
			
			\part $f(x) = \frac{5x - 1}{x^2 - x - 2}$
			\begin{align*}
				f(x) &= \frac{5x -1}{x^2 - x - 2} \\
				&= \frac{5x-1}{(x+1)(x-2)} \\
				&= \frac{2}{x+1} + \frac{3}{x-2} \\
				&= 2 \cdot \sum (-x)^k + 3 \cdot \sum (x+1)^k
			\end{align*}
			
			\part $f(x) = \frac{2}{(1 - 2x)^2}$
			We know that:
			\[
				\frac{2}{(1 - 2x)^2} = \frac{d}{dx} \frac{1}{1-2x}
			\]
			Now, because of \ref{5a}: 
			\[
				f(x) = \frac{d}{dx} = \sum 2k(2x)^k
			\]
			This only converges if $|x| < \frac{1}{2}$.
			
			
		\end{parts} 
	\end{questions}
\end{document}